RocqOfRust/revm/revm_interpreter/instructions/links/bitwise/byte.v
@@ -2,11 +2,13 @@ Require Import RocqOfRust.RocqOfRust.
 Require Import links.RocqOfRust.
 Require Import core.convert.links.num.
 Require Import core.links.cmp.
+Require Import core.links.option.
 Require Import core.links.result.
 Require Import core.num.links.error.
 Require Import core.num.links.mod.
 Require Import revm.revm_interpreter.gas.links.constants.
 Require Import revm.revm_interpreter.links.gas.
+Require Import revm.revm_interpreter.links.instruction_context.
 Require Import revm.revm_interpreter.links.instruction_result.
 Require Import revm.revm_interpreter.links.interpreter.
 Require Import revm.revm_interpreter.links.interpreter_types.
@@ -20,14 +22,17 @@ Instance run_byte
     {WIRE H : Set} `{Link WIRE} `{Link H}
     {WIRE_types : InterpreterTypes.Types.t} `{InterpreterTypes.Types.AreLinks WIRE_types}
     (run_InterpreterTypes_for_WIRE : InterpreterTypes.Run WIRE WIRE_types)
-    (interpreter : '&mut (Interpreter.t WIRE WIRE_types))
-    (_host : '&mut H) :
+    (context : InstructionContext.t H WIRE WIRE_types) :
   Run.Trait
-    instructions.bitwise.byte [] [ Φ WIRE; Φ H ] [ φ interpreter; φ _host ]
+    instructions.bitwise.byte [] [ Φ WIRE; Φ H ] [ φ context ]
     unit.
 Proof.
   constructor.
+  destruct run_InterpreterTypes_for_WIRE eqn:?.
+  destruct run_StackTrait_for_Stack.
+  destruct run_LoopControl_for_Control.
   destruct Impl_TryFrom_u64_for_usize.run.
   run_symbolic.
+  { eapply Impl_Interpreter.run_halt_underflow. }
 Defined.
 Global Opaque run_byte.
